Test/CaseStudies/AATrees.lean
@@ -1,0 +1,90 @@
+import Chako
+
+inductive AATree (α : Type u) where
+  | nil
+  | node (x : α) (level : Nat) (l r : AATree α)
+  deriving Repr
+
+namespace AATree
+
+def lvl : AATree α → Nat
+  | nil => 0
+  | node _ lvl _ _ => lvl
+
+def left : AATree α → AATree α
+  | nil => .nil
+  | node _ _ l _ => l
+
+def right : AATree α → AATree α
+  | nil => .nil
+  | node _ _ _ r => r
+
+def isNil : AATree α → Bool
+  | nil => true
+  | node .. => false
+
+def data (t : AATree α) (h : t.isNil = false := by grind) : α :=
+  match t with
+  | nil => False.elim (by grind [isNil])
+  | node x .. => x
+
+def mem (x : α) : AATree α → Prop
+  | nil => False
+  | node d _ l r => d = x ∨ mem x l ∨ mem x r
+
+def WF : AATree α → Prop
+  | nil => True
+  | node _ lvl nil nil => lvl = 1
+  | node _ lvl l r =>
+    WF l ∧ WF r ∧ lvl ≥ r.lvl ∧ lvl > l.lvl ∧ (lvl > 1 → (!l.isNil ∧ !r.isNil))
+
+def skew : AATree α → AATree α
+  | nil => nil
+  | node x lvl l r =>
+    -- TODO: typo l to r here
+    if h : !l.isNil ∧ lvl = l.lvl then
+      node l.data lvl l.left (node x lvl l.right r)
+    else
+      node x lvl l r
+
+def split : AATree α → AATree α
+  | nil => nil
+  | node x lvl l r =>
+    if h : !r.isNil ∧ lvl = r.right.lvl then
+      node r.data (lvl + 1) (node x lvl l r.left) r.right
+    else
+      node x lvl l r
+
+def insert [LT α] [DecidableLT α] (t : AATree α) (x : α) : AATree α :=
+  match t with
+  | nil => .node x 1 nil nil
+  | node y lvl l r =>
+    let l' := if x < y then l.insert x else l
+    let r' := if x > y then r.insert x else r
+    split <| skew <| node y lvl l' r'
+
+
+section
+
+variable {α : Type u} (t : AATree α)
+
+example : mem x t ↔ t.skew.mem x := by
+  chako
+
+example : mem x t ↔ t.split.mem x := by
+  chako
+
+example : WF t → t.skew = t := by
+  sorry
+  -- timeout chako
+
+example : WF t → t.split = t := by
+  sorry
+  -- timeout chako
+
+end
+
+#eval insert (AATree.node (Nat.succ Nat.zero) (Nat.succ Nat.zero) AATree.nil AATree.nil) 0
+example (t : AATree Nat) : WF t → WF (t.insert x) := by
+  sorry
+  -- timeout chako
